% Agenda:
%   [ ] Thm. induction
%   [ ] Examples of induction

\begin{frame}{Induction from $\N$}
  
  % \begin{block}{Theorem: Vanilla induction}
  %   \par Let $P : \N \to \Bool$ be a predicate on $\N$. If
  %   \begin{align*}
  %     P (0)
  %     \text{ and } (\forall n \in \N,\, P (n) \implies P (\Succ (n)))
  %   \end{align*}
  %   then $\forall n \in \N,\, P(n)$.
  % \end{block}

  % \pause

  \begin{block}{Theorem: Simple induction}
    \par Let $\lhs, \rhs : \N \to X$ be two functions out of $\N$. If
    \begin{itemize}[nosep]
      \item[$\bullet$] $\lhs(0) = \rhs(0)$, and
      \item[$\bullet$] $(\forall n \in \N,\, \lhs(n) = \rhs(n) \implies \lhs( \Succ (n) ) = \rhs ( \Succ (n) ))$
    \end{itemize}
    then $\lhs = \rhs$.
  \end{block}

\end{frame}

\begin{frame}{Induction from $\N$}

  \begin{block}{Theorem: Simple induction}
    \par Let $\lhs, \rhs : \N \to X$ be two functions out of $\N$. If
    \begin{itemize}[nosep]
      \item[$\bullet$] $\lhs(0) = \rhs(0)$, and
      \item[$\bullet$] $(\forall n \in \N,\, \lhs(n) = \rhs(n) \implies \lhs( \Succ (n) ) = \rhs ( \Succ (n) ))$
    \end{itemize}
    then $\lhs = \rhs$.
  \end{block}

  \begin{align*}
    0 + y &:= y 
    & \Succ(x) + y &:= \Succ(x + y)
  \end{align*}

  \pause
  
  \begin{block}{Example: $\forall n \in \N,\, n + 0 = n$}
    
    \pause

    \par Let $\lhs : n \mapsto n + 0$ and $\rhs : n \mapsto n$. Then,
    \pause
    \begin{itemize}[nosep]
      \item[$\bullet$] $\lhs(0) = 0 + 0 = 0 = \rhs(0)$; \pause
      \item[$\bullet$] $\lhs(\Succ(n)) = \Succ(n) + 0 = \Succ(n + 0) \mathbin{\textcolor{magenta}{=}} \Succ(n) = \rhs(\Succ(n))$;
    \end{itemize}
    \pause
    so $\lhs = \rhs$.

  \end{block}

\end{frame}
