% Agenda:
%   [x] $\forall x \in \coN, \pred(x + y) = x + \pred(y)$ whenever $\pred(y) \neq \no$.

\renewcommand{\currentGoal}{$\forall x, y, y' \in \coN$, if $\pred(y) = y' \neq \no$, then $\pred(x + y) = x + y'$}

\begin{frame}[t]{Coinduction into $\coN$} % .;
  \simpleCoindNBlock

  \begin{itemize}
    \item[$(*)$] {
      $\pred(a + b) = \pred(b)$ whenever $\pred(a) = \no$
    }
    \item[$(**)$] {
      $\pred(a + b) = \pred(a) + b$ whenever $\pred(a) \neq \no$
    }
  \end{itemize}

  \vspace{0.5\baselineskip}

  \par\textbf{Proof that \currentGoal.}
  
\end{frame}

\begin{frame}[t]{Coinduction into $\coN$} % .;
  \simpleCoindNBlock

  \vspace{0.5 \baselineskip}

  \par\textbf{Proof that \currentGoal.}
  \vspace{0.5\baselineskip}
  \par Set $X := \set*{(x, y, y') \in \coN^3 \given \pred(y) = y' }$
  \vspace{0.5\baselineskip}
  \par Define $\lhs (x, y, y') := \pred(x + y)$ and $\rhs (x, y, y') := x + y'$.
  
\end{frame}

% \begin{frame}[t]{Coinduction into $\coN$: \currentGoal} % .;
%   \simpleCoindNBlock

%   \begin{itemize}
%     \item[$(**)$] {
%       $\pred(x + y) = \pred(x) + y$ whenever $\pred(x) \neq \no$
%     }
%   \end{itemize}

%   \vspace{0.5 \baselineskip}

%   \par\textbf{Proof that \currentGoal.}
%   \par Set $\lhs : x \mapsto x + 0$ and $\rhs : x \mapsto x$.
%   \begin{itemize}[]
%     \item[$\bullet$] {
%       If instead $\pred(x) \neq \no$, then
%       \begin{align*}
%         [\pred(\lhs(x))]
%         &= \textcolor{red!50!white}{[\pred(x + 0)]}
%         \\
%         &= \textcolor{orange!50!white}{[\pred(x) + 0]}
%         \\
%         &= \textcolor{green}{[\lhs(\pred(x))]}
%         \\
%         &= \textcolor{cyan!50!white}{[\rhs(\pred(x))]}
%         \\
%         &= \textcolor{blue!50!white}{[\pred(x)]}
%         \\
%         [\pred(\lhs(x))]
%         &= \textcolor{pink}{[\pred(\rhs(x))]}
%       \end{align*}
%     }
%   \end{itemize}
  
% \end{frame}

% \begin{frame}[t]{Coinduction into $\coN$} % .;
%   \simpleCoindNBlock

%   \par\textbf{Proof that \currentGoal.}
%   \par Set $\lhs : x \mapsto x + 0$ and $\rhs : x \mapsto x$.
%   \begin{itemize}
%     \item[$\bullet$] {
%       The theorem asserts $\lhs = \rhs$.
%       \qed
%     }
%   \end{itemize}
  
% \end{frame}
