% Agenda:
%   [x] $\forall x, y \in \coN, x + y = y + x$

\renewcommand{\currentGoal}{$\forall x, y \in \coN,\, x + y = y + x$}

\begin{frame}[t]{Coinduction into $\coN$: \currentGoal} % .;
  \simpleCoindNBlock

  \begin{itemize}
    \item[$\bullet$] {
      $\pred(a + b) = \pred(b)$ whenever $\pred(a) = \no$
    }
    \item[$\bullet$] {
      $\pred(a + b) = \pred(a)$ whenever $\pred(b) = \no$
    }
    \item[$\bullet$] {
      $\pred(a + b) = \pred(a) + b$ whenever $\pred(a) \neq \no$
    }
    \item[$\bullet$] {
      $\pred(a + b) = a + \pred(b)$ whenever $\pred(b) \neq \no$ \textcolor{gray}{(possible)}
    }
  \end{itemize}

  \vspace{0.5\baselineskip}

  \par\textbf{Proof that \currentGoal.}
  
\end{frame}

\begin{frame}[t]{Coinduction into $\coN$: \currentGoal} % .;
  \simpleCoindNBlock

  \vspace{0.5 \baselineskip}

  \par\textbf{Proof that \currentGoal.}
  \vspace{0.5 \baselineskip}
  \begin{itemize}
    \item[$\bullet$] {
      Set $X := \coN^2$.
    }
    \item[$\bullet$] {
      Set $\lhs(x, y) := x + y$.
    }
    \item[$\bullet$] {
      Set $\rhs(x, y) := y + x$.
    }
  \end{itemize}

\end{frame}

\begin{frame}[t]{Coinduction into $\coN$: \currentGoal} % .;
  \simpleCoindNBlock

  \begin{itemize}
    \item[$\bullet$] {
      $\pred(a + b) = \pred(b)$ whenever $\pred(a) = \no$
    }
    \item[$\bullet$] {
      $\pred(a + b) = \pred(a)$ whenever $\pred(b) = \no$
    }
  \end{itemize}

  \vspace{0.5 \baselineskip}

  \par\textbf{Proof that \currentGoal.}
  \begin{itemize}
    \item[$\bullet$] {
      If $\pred(x) = \no$, then
      \pause
      \begin{align*}
        [\pred(\lhs(x, y))]
        &= \red{[\pred(x + y)]}
        \\
        &= \orange{[\pred(y)]}
        \\
        &= \green{[\pred(y + x)]}
        \\
        [\pred(\lhs(x, y))]
        &= \cyan{[\pred(\rhs(x, y))]}
      \end{align*}
    }
  \end{itemize}
  
\end{frame}

\begin{frame}[t]{Coinduction into $\coN$: \currentGoal} % .;
  \simpleCoindNBlock

  \begin{itemize}
    \item[$\bullet$] {
      $\pred(a + b) = \pred(a) + b$ whenever $\pred(a) \neq \no$
    }
    \item[$\bullet$] {
      $\pred(a + b) = a + \pred(b)$ whenever $\pred(b) \neq \no$
    }
  \end{itemize}

  \vspace{0.5 \baselineskip}

  \par\textbf{Proof that \currentGoal.}
  \begin{itemize}
    \item[$\bullet$] {
      If $\pred(x) \neq \no$, then
      \pause
      \begin{align*}
        [\pred(\lhs(x, y))]
        &= \red{[\pred(x + y)]}
        \\
        &= \orange{[\pred(x) + y]}
        \\
        &= \green{[\lhs(\pred(x), y)]}
        \\
        &= \cyan{[\rhs(\pred(x), y)]}
        \\
        &= \blue{[y + \pred(x)]}
        \\
        &= \pink{[\pred(y + x)]}
        = [\pred(\rhs(x, y))]
      \end{align*}
    }
  \end{itemize}
  
\end{frame}

\begin{frame}[t]{Coinduction into $\coN$: \currentGoal} % .;
  \simpleCoindNBlock

  \par\textbf{Proof that \currentGoal.}
  \begin{itemize}
    \item[$\bullet$] {
      The theorem asserts $\lhs = \rhs$.
      \qed
    }
  \end{itemize}
  
\end{frame}
